\documentclass{article}
\usepackage{graphicx}
\usepackage{amsmath}

\topmargin=-0.45in
\evensidemargin=0in
\oddsidemargin=0in
\textwidth=6.5in
\textheight=9.0in
\headsep=0.25in


\begin{document}

\title{Complex Analysis}
\author{Josh Cai}

\maketitle  

\section{Chapter 1}
% \input{ch1.tex}
\begin{enumerate}

\item[\textbf{1.7}] 
\textit{(i)}
Let $z = r\mathrm{e}^{\mathrm{i}\theta}$.
\begin{align*}
    z^3+1 &= 0 \\
    z^3   &= -1 \\
    r^3\mathrm{e}^{3\mathrm{i}\theta} &= -1
\end{align*}
Then, $r^3 = |-1|$, so $ r=1$, and we have:
\begin{gather*}
  \cos 3\theta + \mathrm{i} \sin 3\theta = -1 \\
  \cos 3\theta = -1 \\
  3\theta = (2k+1)\pi, \text{for } k = 0, 1, 2, ...
\end{gather*}
So we have $\theta = \pi/3, \pi, 5\pi/3$, therefore 
$z = \mathrm{e}^{\pi/3\mathrm{i}}, \:
-1, \:
\mathrm{e}^{5\pi/3\mathrm{i}}$.
\\\\
\textit{(ii)}
Let $z = r\mathrm{e}^{\mathrm{i}\theta}$.
\begin{align*}
    z^4+1 &= 0 \\
    z^4   &= -1 \\
    r^4\mathrm{e}^{4\mathrm{i}\theta} &= -1
\end{align*}
Then, $r^4 = |-1|$, so $ r=1$, and we have:
\begin{gather*}
  \cos 4\theta + \mathrm{i} \sin 4\theta = -1 \\
  \cos 4\theta = -1 \\
  4\theta = (2k+1)\pi, \text{for } k = 0, 1, 2, ...
\end{gather*}
So we have $\theta = \pi/4, 3\pi/4, 5\pi/4, 7\pi/4$, 
therefore $z = \mathrm{e}^{\pi/4\mathrm{i}}, \:
\mathrm{e}^{3\pi/4\mathrm{i}}, \:
\mathrm{e}^{5\pi/4\mathrm{i}}, \:
\mathrm{e}^{7\pi/4\mathrm{i}}$.
\\\\
\textit{(iii)}
Let $z = r\mathrm{e}^{\mathrm{i}\theta}$.
\begin{align*}
    z^6+1 &= 0 \\
    z^6   &= -1 \\
    r^6\mathrm{e}^{6\mathrm{i}\theta} &= -1
\end{align*}
Then, $r^6 = |-1|$, so $ r=1$, and we have:
\begin{gather*}
  \cos 6\theta + \mathrm{i} \sin 6\theta = -1 \\
  \cos 6\theta = -1 \\
  6\theta = (2k+1)\pi, \text{for } k = 0, 1, 2, ...
\end{gather*}
So we have 
$\theta = \frac{\pi}{6}, \pi/2, 5\pi/6, 7\pi/6, 3\pi/2, 11\pi/6$, 
therefore 
$z = \mathrm{e}^{\pi/6\mathrm{i}}, \:
\mathrm{e}^{\pi/2\mathrm{i}},\:
\mathrm{e}^{5\pi/6\mathrm{i}},\:
\mathrm{e}^{7\pi/6\mathrm{i}},\:
\mathrm{e}^{3\pi/2\mathrm{i}},\:
\mathrm{e}^{11\pi/6\mathrm{i}}
$.

\item[\textbf{1.8}] 
\textit{(i)}
$1+z+...+z^7 = \dfrac{z^8-1}{z-1}$

The solutions of $\dfrac{z^8-1}{z-1} = 0$ are the 8th roots of unity, except for 1. 

So, $z = \mathrm{e}^{\pi/4\mathrm{i}}, \:
\mathrm{e}^{\pi/2\mathrm{i}},\:
\mathrm{e}^{3\pi/4\mathrm{i}},\:
\mathrm{e}^{\pi\mathrm{i}},\:
\mathrm{e}^{5\pi/4\mathrm{i}},\:
\mathrm{e}^{3\pi/2\mathrm{i}}, \:
\mathrm{e}^{7\pi/4\mathrm{i}}
$.
\\\\
\textit{(ii)}
\\\\
\textit{(iii)}
$1-z+z^2 = \dfrac{z^3+1}{z+1}$

The solutions of $\dfrac{z^3+1}{z+1} = 0$ are the solutions of $z^3+1 = 0$ (found in 1.7\textit{(i)}), except for -1. 

So, $z = \mathrm{e}^{\pi/3\mathrm{i}}, \:
\mathrm{e}^{5\pi/3\mathrm{i}}
$.
\\\\
\textit{(iv)}
\\\\

\end{enumerate}
\section{Chapter 2}

\section{Chapter 3}

\end{document}â€‹ 