\begin{enumerate}

\item[\textbf{4.2}] 
\textit{(i)}
Join of: \\
\begin{align*}
&\gamma (t) = (1-t) + \mathrm{i}t, \: t \in [0,1] \\
&\gamma (t) = (1-t)\mathrm{i} - t, \: t \in [0,1] \\
&\gamma (t) = -(1-t) - \mathrm{i}t, \: t \in [0,1] \\
&\gamma (t) = -(1-t)\mathrm{i} + t, \: t \in [0,1]
\end{align*}

\textit{(ii)}
\[\gamma (t) = R\mathrm{e}^{\mathrm{i}t}, \: t \in [-\pi/2,\pi/2] \]

\textit{(iii)}
Join of: \\
\begin{align*}
&\gamma (t) = 1+\mathrm{e}^{\mathrm{i}(4\pi-t)}, \: t \in [\pi,3\pi] \\
&\gamma (t) = -1+\mathrm{e}^{\mathrm{i}t}, \: t \in [0,2\pi] 
\end{align*}

\end{enumerate}